theories/Infra/MoreTac.v
@@ -1,0 +1,22 @@
+Ltac let_unfold id :=
+  cbv beta delta [id];
+  repeat match goal with
+         | [ |- context [ let s := ?e in _ ] ] => set (s:=e)
+         | [ |- context [let (a, b) := ?e in _] ] =>
+           let a := fresh a in let b := fresh b in case_eq e; intros b a ?
+         | [ H : ?x = (?s, ?t) |- _ ] =>
+           assert (fst x = s) by (rewrite H; eauto);
+             assert (snd x = t) by (rewrite H; eauto); clear H
+         | [ |- context f [ let s := ?e in @?t s ] ] =>
+           is_var e;
+             let s := eval cbv beta in (t s) in
+                 let x := context f[s] in
+                 change x
+         end.
+
+Tactic Notation "refold" :=
+  repeat match goal with
+         | [ x := ?e |- context f [ ?e ]] =>
+           let y := context f[x] in
+           change y
+         end.
